Complexitylib/Models.lean
@@ -15,5 +15,6 @@ import Complexitylib.Models.TuringMachine.Subroutines
 import Complexitylib.Models.TuringMachine.CounterSubroutines
 import Complexitylib.Models.TuringMachine.Registers
 import Complexitylib.Models.TuringMachine.Emit
+import Complexitylib.Models.TuringMachine.RegisterOps
 import Complexitylib.Models.TuringMachine.NonDetSubroutines
 import Complexitylib.Models.TuringMachine.Subroutines.Internal
